seiostar/QTypes.HelperTactics.fst
@@ -11,15 +11,14 @@ let simplify_stack_ops () : Tac unit =
 let simplify_qType_g g (x:term) : Tac term =
   norm_term_env g [
     delta_only [
-      `%fs_oval; `%fs_val; `%qUnit; `%qBool; `%qString; `%qResexn;
+      `%fs_oval; `%fs_val; `%qUnit; `%qBool; `%qString; `%qResexn; `%qRef; `%qFileDescr;
       `%op_Hat_Subtraction_Greater; `%op_Hat_Star; `%op_Hat_Plus;
       `%op_Hat_Subtraction_Greater_Bang_At;
       `%get_rel; `%get_Type;
       `%q_io_args; `%q_io_res;
       `%Mkdtuple2?._1;`%Mkdtuple2?._2];
-    zeta;
     iota;
-    simplify
   ] x
+
 
 let simplify_qType (x:term) : Tac term = simplify_qType_g (top_env ()) x
